theory/cwp/cwp_cwpf.v
@@ -12,12 +12,20 @@ Require Import Coq.micromega.Lia.
 Local Open Scope program_scope.
 Import ListNotations.
 
+Require Import ExtLib.Structures.Monad.
+Require Import ExtLib.Structures.MonadState.
+Require Import ExtLib.Data.Monads.StateMonad.
+Require Import ExtLib.Data.Monads.ListMonad.
+
+Require Import compile.
 Require Import cpGCL.
 Require Import cwp.
 Require Import cwpf_infer.
 Require Import geometric.
+Require Import infer.
 Require Import order.
 Require Import Q.
+Require Import tree.
 
 Open Scope cpGCL_scope.
 Open Scope Q_scope.
@@ -35,7 +43,8 @@ Proof.
     intros ?; apply IHc2.
   - destruct (e st); auto.
   - rewrite IHc1, IHc2. lra.
-  - destruct (Qeq_dec (wpf c (fun st => if e st then 1 else 0) st) 1).
+  - destruct (e st); try reflexivity.
+    destruct (Qeq_dec (wpf c (fun st => if e st then 1 else 0) st) 1).
     + rewrite q, Qminus_cancel, 3!Qdiv_0_den; lra.
     + assert (H0: forall a b c, ~ c == 0 -> a / c + b / c == (a + b) / c).
       { intros. field; auto. }
@@ -66,7 +75,8 @@ Proof.
   - unfold compose; auto.
   - destruct (e x); auto.
   - rewrite IHc1, IHc2; auto; lra.
-  - rewrite IHc.
+  - destruct (e x); auto.
+    rewrite IHc.
     + apply Qdiv_0_num.
     + intro y; destruct (e y); auto; reflexivity.
   - destruct (e x); auto; reflexivity.
@@ -90,6 +100,7 @@ Proof.
     assert (eb <= 1).
     { apply IHc; auto.
       intro y; destruct (e y); lra. }
+    destruct (e x); auto.
     destruct (Qeq_dec eb 1).
     { rewrite q, Qminus_cancel, Qdiv_0_den; lra. }
     apply ratio_Qle_sum. lra.
@@ -122,7 +133,8 @@ Proof.
     intros ?; apply IHc2.
   - destruct (e st); auto.
   - rewrite IHc1, IHc2. lra.
-  - destruct (Qeq_dec (wpf c (fun st => if e st then 1 else 0) st) 1).
+  - destruct (e st); try reflexivity.
+    destruct (Qeq_dec (wpf c (fun st => if e st then 1 else 0) st) 1).
     + rewrite Qeq_eq_bool; auto.
       rewrite q, Qminus_cancel, Qdiv_0_den; lra.
     + rewrite Qeq_bool_false; auto.
@@ -161,6 +173,7 @@ Proof.
   - specialize (IHc1 f H3 Hle x); specialize (IHc2 f H4 Hle x); nra.
   - set (ea := wlpf c (fun st => if e st then 0 else f st) x).
     set (eb := wpf c (fun st => if e st then 1 else 0) x).
+    destruct (e x); auto.
     assert (eb <= 1).
     { apply wpf_bounded; auto.
       intro y; destruct (e y); lra. }
@@ -184,6 +197,38 @@ Proof.
   - destruct (e x); auto; lra.
 Qed.
 
+Lemma wpf_disjoint_le_1 c (e : exp) st :
+  wf_cpGCL c ->
+  wpf c (fun x => if e x then 1 else 0) st +
+  wpf c (fun x => if e x then 0 else 1) st <= 1.
+Proof.
+  intros Hwf.
+  set (a := wpf c (fun st : St => if e st then 1 else 0) st).
+  set (b := wpf c (fun st : St => if e st then 0 else 1) st).
+  assert (a == wpf c (fun x => if e x then const 1 x else 0) st).
+  { apply Proper_wpf; auto. intro y; destruct (e y); reflexivity. }
+  rewrite H. unfold b.
+  rewrite <- wpf_linear'.
+  apply wpf_bounded; auto.
+  intro y; destruct (e y); auto; unfold const; lra.
+Qed.
+
+Lemma wlpf_disjoint_le_1 c (e : exp) st :
+  wf_cpGCL c ->
+  wpf c (fun x => if e x then 1 else 0) st +
+  wlpf c (fun x => if e x then 0 else 1) st <= 1.
+Proof.
+  intros Hwf.
+  set (a := wpf c (fun st : St => if e st then 1 else 0) st).
+  set (b := wlpf c (fun st : St => if e st then 0 else 1) st).
+  assert (a == wpf c (fun x => if e x then const 1 x else 0) st).
+  { apply Proper_wpf; auto. intro y; destruct (e y); reflexivity. }
+  rewrite H. unfold b.
+  rewrite <- wlpf_linear'.
+  apply wlpf_bounded; auto.
+  intro y; destruct (e y); auto; unfold const; lra.
+Qed.
+
 Lemma wpf_expectation c f :
   wf_cpGCL c ->
   expectation f ->
@@ -201,6 +246,7 @@ Proof.
     specialize (IHc1 f H3 Hexp x); specialize (IHc2 f H4 Hexp x).
     nra.
   - intro x. simpl.
+    destruct (e x); auto.
     assert (wpf c (fun st => if e st then 1 else 0) x <= 1).
     { apply wpf_bounded; auto.
       intro st; destruct (e st); auto; lra. }
@@ -228,6 +274,7 @@ Proof.
     specialize (IHc1 f H3 Hexp x); specialize (IHc2 f H4 Hexp x).
     nra.
   - intro x. simpl.
+    destruct (e x); auto.
     assert (wpf c (fun st => if e st then 1 else 0) x <= 1).
     { apply wpf_bounded; auto.
       intro st; destruct (e st); auto; lra. }
@@ -244,30 +291,12 @@ Lemma wlpf_bounded_expectation c f :
   bounded_expectation f ->
   bounded_expectation (wlpf c f).
 Proof.
-  revert f.
-  induction c; intros f Hwf Hexp; simpl; inversion Hwf; subst; auto.
-  - unfold const; intros ?; lra.
-  - intros ?; apply Hexp.
-  - apply IHc1; auto.
-  - intro x; destruct (e x).
-    + apply IHc1; auto.
-    + apply IHc2; auto.
-  - intro x.
-    specialize (IHc1 f H3 Hexp x); specialize (IHc2 f H4 Hexp x).
-    nra.
-  - intro x. simpl.
-    assert (wpf c (fun st => if e st then 1 else 0) x <= 1).
-    { apply wpf_bounded; auto.
-      intro st; destruct (e st); auto; lra. }
-    destruct (Qeq_dec (wpf c (fun st => if e st then 1 else 0) x) 1).
-    + apply Qeq_bool_iff in q. rewrite q; lra.
-    + rewrite Qeq_bool_false; auto; split.
-      * apply Qle_shift_div_l. lra.
-        rewrite Qmult_0_l; apply IHc; auto.
-        intro st; destruct (e st); auto; lra.
-      * admit.
-  - intro x; destruct (e x); auto; lra.
-Admitted.
+  intros Hwf Hf x; split.
+  - apply wlpf_expectation; auto.
+    intro y; apply Hf.
+  - apply wlpf_bounded; auto.
+    intro y; apply Hf.
+Qed.
 
 Lemma wpf_chain_geometric_series f e c st i :
   iid_wpf e c ->
@@ -288,16 +317,10 @@ Lemma wlpf_chain_series f e c st i :
   wlpf (unroll e c i) f st ==
   wlpf_series (wlpf c (fun x => if e x then 0 else f x) st)
               (wpf c (indicator e) st) i.
-  (* geometric_series'' (wlpf c (fun x => if e x then 0 else f x) st) *)
-  (*                    (wpf c (indicator e) st) i + *)
-  (* Qpow (wpf c (indicator e) st) i. *)
 Proof.
   unfold wlpf_series; intro Hiid; induction i.
   - reflexivity.
-  - rewrite Hiid, IHi, Qplus_comm.
-    simpl.
-    (* set (a := wlpf c (fun x : St => if e x then 0 else f x) st). *)
-    (* set (r := wpf c (indicator e) st). *)
+  - rewrite Hiid, IHi, Qplus_comm; simpl.
     rewrite Qmult_plus_distr_r, Qplus_assoc, geometric_series''_succ.
     reflexivity.
 Qed.
@@ -306,11 +329,6 @@ Lemma wf_unroll c e i :
   wf_cpGCL c ->
   wf_cpGCL (unroll e c i).
 Proof. induction i; repeat constructor; auto. Qed.
-
-(* Lemma kdfgfsdf c e st : *)
-(*   wf_cpGCL c -> *)
-(*   wpf c (indicator e) st + wpf c (neg_indicator e) st == 1. *)
-(* Admitted. *)
 
 Lemma wpf_monotone c :
   wf_cpGCL c ->
@@ -326,7 +344,8 @@ Proof.
   - specialize (IHc1 H3 f g Hleq x).
     specialize (IHc2 H4 f g Hleq x).
     unfold leq in *; simpl in *; nra.
-  - specialize (IHc H0).
+  - destruct (e x); auto.
+    specialize (IHc H0).
     cut (wpf c (fun st' : St => if e st' then 0 else f st') x <=
          wpf c (fun st' : St => if e st' then 0 else g st') x).
     { intros.
@@ -342,66 +361,39 @@ Proof.
   - destruct (e x); auto; lra.
 Qed.
 
-(* Lemma wpf_decreasing c f x : *)
-(*   wpf c f x <= f x. *)
-(* Proof. *)
-(*   (* revert f x. *) *)
-(*   (* induction c; intros f x Hexp; simpl. *) *)
-(*   (* - lra. *) *)
-(*   (* - apply Hexp. *) *)
-(*   (* -  *) *)
-(* Admitted. *)
-
-(* Lemma kdfgf c e st : *)
-(*   wf_cpGCL c -> *)
-(*   (forall f, f ==f indicator e -> wpf c f st == 1) -> *)
-(*   (* forall g, g ==f neg_indicator e -> wpf c g st == 0. *) *)
-(*   forall f g, expectation g -> (forall x, g x <= if e x then 0 else f x) -> *)
-(*          wpf c g st == 0. *)
-(* Proof. *)
-(*   revert e st. *)
-(*   induction c; intros G st Hwf Heq f g Hexp Hle. *)
-(*   - simpl in *. *)
-(*     specialize (Heq (indicator G) (f_Qeq_refl _)). *)
-(*     unfold indicator in *. *)
-(*     (* rewrite Heq'. *) *)
-(*     specialize (Hle st). *)
-(*     destruct (G st). *)
-(*     + specialize (Hexp st); lra. *)
-(*     + lra. *)
-(*   - reflexivity. *)
-(*   - simpl in *. admit. *)
-(*   - simpl in *. *)
-(*     unfold compose in *. *)
-(*     inversion Hwf; subst. *)
-(*     apply IHc1 with (e:=G) (f:=f); auto. *)
-(*     + intros h Hh. *)
-(*       specialize (Heq h Hh). *)
-(*       assert (Hle': 1 <= wpf c1 h st). *)
-(*       { apply Qle_trans with (wpf c1 (wpf c2 h) st). *)
-(*         - lra. *)
-(*         - apply wpf_monotone; auto. *)
-(*           intro s; simpl. *)
-(*           apply wpf_decreasing. } *)
-(*       assert (wpf c1 h st <= 1). *)
-(*       { apply wpf_bounded; auto. *)
-(*         intro y. rewrite Hh. unfold indicator. destruct (G y); lra. } *)
-(*       lra. *)
-(*     + apply wpf_expectation; auto. *)
-(*     + intro x; specialize (Hle x). *)
-(*       apply Qle_trans with (g x); auto. *)
-(*       apply wpf_decreasing. *)
-(*   - admit. (* TODO *) *)
-(*   - admit. *)
-(*   - admit. *)
-(*   - simpl in *. *)
-(*     specialize (Heq (indicator G) (f_Qeq_refl _)). *)
-(*     unfold indicator in Heq. *)
-(*     destruct (e st); try lra. *)
-(*     specialize (Hle st). destruct (G st). *)
-(*     + specialize (Hexp st); lra. *)
-(*     + lra. *)
-(* Admitted. *)
+Lemma wlpf_monotone c :
+  wf_cpGCL c ->
+  monotone (wlpf c).
+Proof.
+  induction c; unfold monotone, leq; simpl;
+    intros Hwf f g Hleq x; auto; inversion Hwf; subst.
+  - lra.
+  - apply IHc1; auto; apply IHc2; auto.
+  - destruct (e x).
+    + apply IHc1; auto.
+    + apply IHc2; auto.
+  - specialize (IHc1 H3 f g Hleq x).
+    specialize (IHc2 H4 f g Hleq x).
+    unfold leq in *; simpl in *; nra.
+  - destruct (e x); auto.
+    destruct (Qeq_dec (wpf c (fun st' : St => if e st' then 1 else 0) x) 1).
+    { rewrite q; simpl; lra. }
+    rewrite Qeq_bool_false; auto.
+    specialize (IHc H0).
+    cut (wlpf c (fun st' : St => if e st' then 0 else f st') x <=
+         wlpf c (fun st' : St => if e st' then 0 else g st') x).
+    { intros.
+      destruct (Qeq_dec (wpf c (fun x => if e x then 1 else 0) x) 1).
+      { rewrite q, Qminus_cancel, 2!Qdiv_0_den; lra. }
+      assert (wpf c (fun x => if e x then 1 else 0) x <= 1).
+      { apply wpf_bounded; auto.
+        intro y; destruct (e y); lra. }
+      apply Qle_Qdiv; auto.
+      lra. }
+    apply IHc; simpl.
+    intro y; destruct (e y); auto; lra.
+  - destruct (e x); auto; lra.
+Qed.
 
 Lemma asdkdf c (e : exp) st :
   wf_cpGCL c ->
@@ -421,110 +413,74 @@ Proof.
     { apply wpf_expectation; auto.
       intro y; destruct (e y); auto; lra. }
     lra. }
-  assert (a == wpf c (fun x => if e x then const 1 x else 0) st).
-  { apply Proper_wpf; auto. intro y; destruct (e y); reflexivity. }
-  rewrite H. unfold b.
-  rewrite <- wpf_linear'.
-  apply wpf_bounded; auto.
-  intro y; destruct (e y); auto; unfold const; lra.
+  apply wpf_disjoint_le_1; auto.
 Qed.
 
-(* Lemma sdfasdfsdkdf c (e : exp) f st : *)
-(*   wpf c (fun x => if e x then 1 else 0) st == 0 -> *)
-(*   wpf c (fun x => if e x then f x else 0) st == 0. *)
-(* Proof. *)
-
-
-(* Lemma djkifg c f g st : *)
-(*   wpf c f st == 0 -> *)
-(*   wpf c (fun x => f st * g st) st == 0. *)
-(* Proof. *)
-(*   revert f g st. *)
-(*   induction c; simpl; intros f g st Heq; auto. *)
-(*   - rewrite Heq; lra. *)
-(*   -  *)
-
-
-(* Lemma djkifg c (e : exp) f st : *)
-(*   wpf c (fun x => if e x then 0 else f x) st == *)
-(*   wpf c (fun x => if e x then 0 else 1) st * wpf c f st. *)
-(* Proof. *)
-  
-
-Lemma sdfasdkdf c (e : exp) f st :
-  wpf c (fun x => if e x then 0 else 1) st == 0 ->
+Lemma wpf_indicator_1_f_0 c (e : exp) f st :
+  wf_cpGCL c ->
+  wpf c (fun x => if e x then 1 else 0) st == 1 ->
   wpf c (fun x => if e x then 0 else f x) st == 0.
 Proof.
-Admitted.
+  intros Hwf Heq.
+  rewrite wpf_infer_f with (n:=O); auto.
+  rewrite wpf_infer_f with (n:=O) in Heq; auto.
+  unfold compose, evalCompile, evalState in *.
+  destruct (runState (compile c) O) eqn:Hc. simpl in *.
+  assert (Hnotbound: not_bound_in (S n) (t st)).
+  { apply bound_in_not_bound_in; intro HC.
+    eapply compile_bound_labels in HC; eauto; lia. }
+  assert (Hnotin: not_in (S n) (t st)).
+  { apply not_in_not_bound_and_not_free. split; auto.
+    apply free_in_not_free_in; intro HC.
+    eapply compile_free_in_0 in HC; eauto; lia. }
+  assert (Hwft: wf_tree' (t st)).
+  { eapply compile_wf_tree'; eauto. }
+  rewrite <- infer_fail_tree_bind_infer_f with (m := S n) in Heq; auto.
+  + apply (infer_f_fail f) in Heq.
+    * rewrite <- infer_f_bind_fail_f_neg; eauto.
+    * apply wf_tree_bind.
+      ++ intros ? y; destruct (e y); constructor.
+      ++ apply wf_tree'_wf_tree; auto.
+      ++ intros y; destruct (e y); constructor.
+    * apply bound_in_not_bound_in; intro HC.
+      apply bound_in_bind in HC. destruct HC.
+      ++ apply bound_in_not_bound_in in Hnotbound; congruence.
+      ++ destruct H as [y Hbound].
+         destruct (e y); inversion Hbound.
+Qed.
 
-(* Lemma asdkdfgf c e st f : *)
-(*   wf_cpGCL c -> *)
-(*   expectation f -> *)
-(*   wpf c (indicator e) st == 1 -> *)
-(*   wpf c (fun x => if e x then 0 else f x) st == 0. *)
-(* Proof. *)
-(*   unfold indicator. *)
-(*   set (a := wpf c (fun st : St => if e st then 1 else 0) st). *)
-(*   set (b := wpf c (fun st : St => if e st then 0 else f st) st). *)
-(*   intros Hwf Hexp Heq. *)
-(*   cut (a + b <= 1). *)
-(*   { intros. *)
-(*     assert (0 <= a). *)
-(*     { apply wpf_expectation; auto. *)
-(*       intro y; destruct (e y); lra. } *)
-(*     assert (0 <= b). *)
-(*     { apply wpf_expectation; auto. *)
-(*       intro y; destruct (e y); auto; lra. } *)
-(*     lra. } *)
-(*   (* wpf_linear' *) *)
-(*   assert (a == wpf c (fun x => if e x then const 1 x else 0) st). *)
-(*   { apply Proper_wpf; auto. intro y; destruct (e y); reflexivity. } *)
-(*   rewrite H. unfold b. *)
-(*   rewrite <- wpf_linear'. *)
-(*   apply wpf_bounded; auto. *)
-(*   intro y; destruct (e y); auto. *)
-  
-(*   revert e st f. *)
-(*   induction c; simpl; unfold indicator; *)
-(*     intros G st f Hwf Heq; inversion Hwf; subst. *)
-(*   - intro H; destruct (G st); lra. *)
-(*   - intro H; inversion H. *)
-(*   - intro H; destruct (G (upd n (e st) st)); lra. *)
-(*   - unfold compose. intro H. *)
-
-(*   (* revert e st f. *) *)
-(*   (* induction c; simpl; unfold indicator; intros G st f Hwf Heq. *) *)
-(*   (* assert (H0: forall x, indicator G x == (if G x then 1 else 0)). *) *)
-(*   (* { intros; reflexivity. } *) *)
-(*   (* - (* specialize (Heq (indicator G) H0). *) *) *)
-(*   (*   (* unfold indicator in Heq. *) *) *)
-(*   (*   destruct (G st); lra. *) *)
-(*   (* - reflexivity. *) *)
-(*   (* - destruct (G (upd n (e st) st)); lra. *) *)
-(*   (* - unfold compose in *. *) *)
-(*   (*   inversion Hwf; subst. *) *)
-(*   (*   apply kdfgf with (e:=G); auto. *) *)
-(*   (*   intros. *) *)
-(*   (*   rewrite <- Heq. *) *)
-(*   (*   apply Proper_wpf; auto. *) *)
-(*   (*   intro. rewrite H. unfold indicator. *) *)
-(*   (*   apply Heq. *) *)
-(*   intros Hwf Hexp Heq. *)
-(*   apply kdfgf with (e:=e) (f:=f); auto. *)
-(*   - intros g Heq'. *)
-(*     rewrite <- Heq. *)
-(*     eapply Proper_wpf; auto. *)
-(*   - intro x.  *)
-(*     destruct (e x); auto; lra. *)
-(*   - intro; lra. *)
-(* Qed. *)
-
-Lemma asdkdfgf' c e st f :
+Lemma wlpf_indicator_1_f_0 c (e : exp) f st :
   wf_cpGCL c ->
-  (wpf c (indicator e) st == 1) ->
+  wpf c (fun x => if e x then 1 else 0) st == 1 ->
   wlpf c (fun x => if e x then 0 else f x) st == 0.
 Proof.
-Admitted.
+  intros Hwf Heq.
+  rewrite wlpf_infer_f_lib with (n:=O); auto.
+  rewrite wpf_infer_f with (n:=O) in Heq; auto.
+  unfold compose, evalCompile, evalState in *.
+  destruct (runState (compile c) O) eqn:Hc. simpl in *.
+  assert (Hnotbound: not_bound_in (S n) (t st)).
+  { apply bound_in_not_bound_in; intro HC.
+    eapply compile_bound_labels in HC; eauto; lia. }
+  assert (Hnotin: not_in (S n) (t st)).
+  { apply not_in_not_bound_and_not_free. split; auto.
+    apply free_in_not_free_in; intro HC.
+    eapply compile_free_in_0 in HC; eauto; lia. }
+  assert (Hwft: wf_tree' (t st)).
+  { eapply compile_wf_tree'; eauto. }
+  rewrite <- infer_fail_tree_bind_infer_f with (m := S n) in Heq; auto.
+  + apply (infer_f_lib_fail f) in Heq.
+    * rewrite <- infer_f_lib_bind_fail_f_neg; eauto.
+    * apply wf_tree_bind.
+      ++ intros ? y; destruct (e y); constructor.
+      ++ apply wf_tree'_wf_tree; auto.
+      ++ intros y; destruct (e y); constructor.
+    * apply bound_in_not_bound_in; intro HC.
+      apply bound_in_bind in HC. destruct HC.
+      ++ apply bound_in_not_bound_in in Hnotbound; congruence.
+      ++ destruct H as [y Hbound].
+         destruct (e y); inversion Hbound.
+Qed.
 
 Lemma wpf_unroll_const_0 c e x i f :
   wf_cpGCL c ->
@@ -539,8 +495,7 @@ Proof.
   - rewrite Hiid.
     rewrite IHi; auto.
     unfold const. rewrite Qmult_0_r, Qplus_0_l.
-    apply sdfasdkdf; auto.
-    apply asdkdf; auto.
+    apply wpf_indicator_1_f_0; auto.
 Qed.
 
 Lemma wlpf_unroll_const_1 c e x i f :
@@ -554,7 +509,39 @@ Proof.
   - reflexivity.
   - rewrite Hiid. rewrite IHi; auto.
     unfold const. rewrite Qmult_1_r.
-    rewrite Heq. rewrite asdkdfgf'; auto; lra.
+    rewrite Heq. rewrite wlpf_indicator_1_f_0; auto; reflexivity.
+Qed.
+
+Lemma wpf_unroll_chain c e f x :
+  wf_cpGCL c ->
+  expectation f ->
+  chain (fun i => wpf (unroll e c i) f x).
+Proof.
+  intros Hwf Hexp i; simpl; revert x.
+  induction i; intro x; simpl.
+  - unfold const, compose.
+    destruct (e x).
+    + apply wpf_expectation; auto.
+      intro y; lra.
+    + apply Hexp.
+  - destruct (e x); try lra.
+    apply wpf_monotone; auto.
+Qed.
+
+Lemma wlpf_unroll_dec_chain c e f x :
+  wf_cpGCL c ->
+  bounded_expectation f ->
+  dec_chain (fun i => wlpf (unroll e c i) f x).
+Proof.
+  intros Hwf Hexp i; simpl; revert x.
+  induction i; intro x; simpl.
+  - unfold const, compose.
+    destruct (e x).
+    + apply wlpf_bounded; auto; intros; lra.
+    + apply Hexp.
+  - destruct (e x); try lra.
+    unfold compose in *.
+    apply wlpf_monotone; auto.
 Qed.
 
 (** wp and wpf coincide when every loop in the program is iid. *)
@@ -586,25 +573,34 @@ Proof.
       * intro x. unfold ch. unfold compose. unfold flip.
         simpl. reflexivity.
     + apply supremum_pointwise; intro x.
-      assert (Hle: wpf c (indicator e) x <= 1).
-      { apply wpf_bounded; auto.
-        intro y; unfold indicator; destruct (e y); lra. }
-      destruct (Qeq_dec (wpf c (indicator e) x) 1).
-      -- unfold indicator in *.
-         eapply Proper_supremum_Q.
-         rewrite q, Qminus_cancel, Qdiv_0_den; reflexivity.
-         intro i. unfold app_chain, flip.
-         unfold ch. unfold compose, flip.
-         destruct H5; apply wpf_unroll_const_0; auto.
-         apply const_supremum.
-         intro i; unfold const. apply Qeq_equ; reflexivity.
-      -- apply geometric''_supremum.
-           ++ apply wpf_expectation; auto.
+      destruct (e x) eqn:He.
+      * assert (Hle: wpf c (indicator e) x <= 1).
+        { apply wpf_bounded; auto.
+          intro y; unfold indicator; destruct (e y); lra. }
+        destruct (Qeq_dec (wpf c (indicator e) x) 1).
+        ++ unfold indicator in *.
+           eapply Proper_supremum_Q.
+           rewrite q, Qminus_cancel, Qdiv_0_den; reflexivity.
+           intro i. unfold app_chain, flip.
+           unfold ch. unfold compose, flip.
+           destruct H5; apply wpf_unroll_const_0; auto.
+           apply const_supremum.
+           intro i; unfold const. apply Qeq_equ; reflexivity.
+        ++ apply geometric''_supremum.
+           ** apply wpf_expectation; auto.
               intro y; destruct (e y); auto; lra.
-           ++ apply wpf_expectation; auto.
+           ** apply wpf_expectation; auto.
               intro y; destruct (e y); auto; lra.
-           ++ unfold indicator in *; lra.
-           ++ intro i; destruct H5; apply wpf_chain_geometric_series; auto.
+           ** unfold indicator in *; lra.
+           ** intro i; destruct H5; apply wpf_chain_geometric_series; auto.
+      * unfold app_chain. unfold flip. unfold ch. unfold compose, flip.
+        apply const_supremum'.
+        ++ apply wpf_unroll_chain; auto.
+        ++ exists (S 0).
+           intros n Hle.
+           apply Qeq_equ.
+           destruct n. lia.
+           simpl. rewrite He. reflexivity.
 Qed.
 
 (** wlp and wlpf coincide when every loop in the program is iid. *)
@@ -637,35 +633,45 @@ Proof.
       * intro x. unfold ch. unfold compose. unfold flip.
         simpl. reflexivity.
     + apply infimum_pointwise; intro x.
-      assert (Hle: wpf c (indicator e) x <= 1).
-      { apply wpf_bounded; auto.
-        intro y; unfold indicator; destruct (e y); lra. }
-      destruct (Qeq_dec (wpf c (indicator e) x) 1).
-      -- unfold indicator in *.
-         eapply Proper_infimum_Q.
-         rewrite Qeq_eq_bool. reflexivity. auto.
-         intro i. unfold app_chain, ch, flip, compose.
-         destruct H5; apply wlpf_unroll_const_1; auto.
-         apply const_infimum.
-         intro; apply Qeq_equ; reflexivity.
-      -- eapply Proper_infimum_Q. rewrite Qeq_bool_false; auto.
-         reflexivity. reflexivity.
-         apply wlpf_infimum.
-         ++ apply wlpf_expectation; auto.
-            intro y; destruct (Hexp y); destruct (e y); auto; lra.
-         ++ apply wpf_expectation; auto.
-            intro y; destruct (Hexp y); destruct (e y); auto; lra.
-         ++ unfold indicator in *; lra.
-         ++ set (a := wlpf c (fun st' : St => if e st' then 0 else f st') x).
-            set (b := wpf c (fun st' : St => if e st' then 1 else 0) x).
-            assert (H: b == wpf c (fun y => if e y then const 1 y else 0) x).
-            { eapply Proper_wpf; auto. intro y; destruct (e y); reflexivity. }
-            rewrite H; clear H.
-            rewrite Qplus_comm; unfold a.
-            rewrite <- wlpf_linear'.
-            apply wlpf_bounded; auto.
-            intro y; destruct (Hexp y); destruct (e y); auto; unfold const; lra.
-         ++ intro i; destruct H5; apply wlpf_chain_series; auto.
+      destruct (e x) eqn:He.
+      * assert (Hle: wpf c (indicator e) x <= 1).
+        { apply wpf_bounded; auto.
+          intro y; unfold indicator; destruct (e y); lra. }
+        destruct (Qeq_dec (wpf c (indicator e) x) 1).
+        ++ unfold indicator in *.
+           eapply Proper_infimum_Q.
+           rewrite Qeq_eq_bool. reflexivity. auto.
+           intro i. unfold app_chain, ch, flip, compose.
+           destruct H5; apply wlpf_unroll_const_1; auto.
+           apply const_infimum.
+           intro; apply Qeq_equ; reflexivity.
+        ++ eapply Proper_infimum_Q. rewrite Qeq_bool_false; auto.
+           reflexivity. reflexivity.
+           apply wlpf_infimum.
+           ** apply wlpf_expectation; auto.
+              intro y; destruct (Hexp y); destruct (e y); auto; lra.
+           ** apply wpf_expectation; auto.
+              intro y; destruct (Hexp y); destruct (e y); auto; lra.
+           ** unfold indicator in *; lra.
+           ** set (a := wlpf c (fun st' : St => if e st' then 0 else f st') x).
+              set (b := wpf c (fun st' : St => if e st' then 1 else 0) x).
+              assert (H: b == wpf c (fun y => if e y then const 1 y else 0) x).
+              { eapply Proper_wpf; auto. intro y; destruct (e y); reflexivity. }
+              rewrite H; clear H.
+              rewrite Qplus_comm; unfold a.
+              rewrite <- wlpf_linear'.
+              apply wlpf_bounded; auto.
+              intro y; destruct (Hexp y); destruct (e y);
+                auto; unfold const; lra.
+           ** intro i; destruct H5; apply wlpf_chain_series; auto.
+      * apply const_infimum'.
+        ++ apply wlpf_unroll_dec_chain; auto.
+        ++ exists (S O).
+           intros n Hle.
+           destruct n.
+           ** lia.
+           ** unfold app_chain, ch, flip, compose; simpl.
+              rewrite He; reflexivity.
 Qed.
 
 Theorem cwp_cwpf (c : cpGCL) (f : St -> Q) :
