theory/cwp/infer.v
@@ -257,60 +257,80 @@ Proof.
         destruct (Nat.eqb_spec m' n); subst. constructor. constructor; auto.
 Qed.
 
+Lemma not_in_infer_fail_tree_bind {A B : Type} (t : tree A) m (k : A -> tree B) :
+  (forall x, not_in m (k x)) ->
+  (forall n x, bound_in n t -> not_in n (k x)) ->
+  infer_fail m (tree_bind t k) == infer_fail m t.
+Proof.
+  revert m k.
+  induction t; intros m k Hnotin Hnotin'; unfold tree_bind in *; simpl.
+  - apply not_in_infer_fail; auto.
+  - reflexivity.
+  - rewrite IHt1; auto. rewrite IHt2; auto. reflexivity.
+    + intros n x Hbound; apply Hnotin'; solve [constructor; auto].
+    + intros n x Hbound; apply Hnotin'; solve [constructor; auto].
+  - rewrite IHt; auto. rewrite IHt; auto. reflexivity.
+    + intro x; apply Hnotin'; constructor.
+    + intros l x Hbound. apply Hnotin'.
+      destruct (Nat.eqb_spec l n); subst; constructor; auto.
+    + intros l x Hbound. apply Hnotin'.
+      destruct (Nat.eqb_spec l n); subst; constructor; auto.
+Qed.
+
+(* Lemma infer_f_lib_bind_lem1 {A B : Type} n (t : tree A) (k : A -> tree B) : *)
+(*   (forall m x, bound_in m (Fix n t) -> not_in m (k x)) -> *)
+(*   infer_fail n t == 1 -> *)
+(*   infer_fail n (tree_bind t k) == 1. *)
+(* Proof. *)
+(*   intros Hnotin Heq1. *)
+(*   rewrite not_in_infer_fail_tree_bind; auto. *)
+(*   - intro x; apply Hnotin; constructor. *)
+(*   - intros m x Hbound; apply Hnotin. *)
+(*     destruct (Nat.eqb_spec m n); subst; constructor; auto. *)
+(* Qed. *)
+
+Lemma infer_f_lib_bind_lem1 {A B : Type} n (t : tree A) (k : A -> tree B) :
+  (forall m x, bound_in m (Fix n t) -> not_in m (k x)) ->
+  infer_fail n (tree_bind t k) == infer_fail n t.
+Proof.
+  intros Hnotin.
+  rewrite not_in_infer_fail_tree_bind; auto.
+  - reflexivity.
+  - intro x; apply Hnotin; constructor.
+  - intros m x Hbound; apply Hnotin.
+    destruct (Nat.eqb_spec m n); subst; constructor; auto.
+Qed.
+
 Lemma infer_f_lib_bind {A B : Type} (f : B -> Q) (t : tree A) (k : A -> tree B) :
   (forall n x, bound_in n t -> not_in n (k x)) ->
   infer_f_lib (infer_f_lib f ∘ k) t == infer_f_lib f (tree_bind t k).
 Proof.
-  revert f k. induction t; intros f k Hnotin; try reflexivity.
-  - simpl; rewrite IHt1, IHt2; try reflexivity;
+  revert f k. induction t; intros f k Hnotin; simpl; try reflexivity.
+  - rewrite IHt1, IHt2; try reflexivity;
       intros n st Hbound; apply Hnotin;
         try solve [apply bound_in_choice2; auto]; constructor; auto.
-  - simpl.
-    destruct (Qeq_dec (infer_fail n t) 1).
+  - destruct (Qeq_dec (infer_fail n t) 1).
     { rewrite q; simpl.
       destruct (Qeq_dec (infer_fail n (tree_bind t k)) 1).
       { rewrite q0; simpl; reflexivity. }
-      (* rewrite Qeq_bool_false; auto. *)
-      (* TODO: q and n0 are contradictory because q implies infer_fail
-         n (bind t k) == 1 for any k. *)
-      admit. }
+      rewrite infer_f_lib_bind_lem1 in n0; auto; congruence. }
     destruct (Qeq_dec (infer_fail n (tree_bind t k)) 1).
     { rewrite q. simpl.
       rewrite Qeq_bool_false; auto.
       rewrite IHt.
-      - admit.
+      - rewrite infer_f_lib_bind_lem1 in q; auto; congruence.
       - intros m x Hbound; apply Hnotin.
         destruct (Nat.eqb_spec m n); subst; constructor; auto. }
     rewrite 2!Qeq_bool_false; auto.
     rewrite IHt; auto.
-    + admit.
+    + unfold tree_bind. erewrite <- not_in_infer_fail_tree_bind.
+      * reflexivity.
+      * intro x; apply Hnotin; constructor.
+      * intros m x Hbound; apply Hnotin.
+        destruct (Nat.eqb_spec m n); subst; constructor; auto.
     + intros m x Hbound; apply Hnotin.
       destruct (Nat.eqb_spec m n); subst; constructor; auto.
-Admitted.
-      
-(*     apply Qeq_Qdiv. *)
-(*     + apply IHt; intros n0 st Hbound; apply Hnotin. *)
-(*       destruct (Nat.eqb_spec n0 n); subst; constructor; auto. *)
-(*     + apply Qeq_Qminus; try reflexivity. *)
-(*       clear IHt. revert Hnotin. revert k n. induction t; intros k m Hnotin. *)
-(*       * simpl. rewrite not_in_infer_fail. reflexivity. apply Hnotin. constructor. *)
-(*       * simpl. reflexivity. *)
-(*       * simpl. rewrite IHt1, IHt2. reflexivity. *)
-(*         intros m' x Hbound. apply Hnotin. inversion Hbound; subst. *)
-(*         constructor. constructor; auto. apply bound_in_choice2; auto. *)
-(*         intros m' x Hbound. apply Hnotin. inversion Hbound; subst. *)
-(*         constructor. constructor; auto. constructor; auto. *)
-(*       * simpl. rewrite IHt. rewrite IHt. reflexivity. *)
-(*         intros m' x Hbound. apply Hnotin. *)
-(*         inversion Hbound; subst. *)
-(*         destruct (Nat.eqb_spec n m); subst. constructor. constructor; auto. *)
-(*         destruct (Nat.eqb_spec m' m); subst. constructor. constructor; auto. *)
-(*         intros m' x Hbound. apply Hnotin. *)
-(*         inversion Hbound; subst. *)
-(*         constructor. *)
-(*         constructor; auto. *)
-(*         destruct (Nat.eqb_spec m' n); subst. constructor. constructor; auto. *)
-(* Qed. *)
+Qed.
 
 Lemma infer_fail_fbind {A : Type} (t1 t2  : tree A) (l m : nat) :
   l <> m ->
@@ -946,6 +966,78 @@ Proof.
   - simpl; unfold flip; rewrite Heq; reflexivity.
 Qed.
 
+Lemma infer_f_lib_fail_aux {A : Type} (t : tree A) (f : A -> Q) (m : nat) (l : list nat) :
+  wf_tree t ->
+  (forall x : nat, In x l -> not_bound_in x t) ->
+  NoDup l ->
+  not_bound_in m t ->
+  sum_Q_list (map (flip infer_fail t) l) == 1 ->
+  infer_f_lib f t == 0.
+Proof.
+  revert l. induction t; simpl; intros l Hwf Hin_notbound Hnodup Hnotbound Hsum.
+  - rewrite sum_Q_list_map_const_0 in Hsum; inversion Hsum.
+  - reflexivity.
+  - inversion Hwf; inversion Hnotbound; subst.
+    destruct (Qeq_dec q 0).
+    + rewrite q0. rewrite Qmult_0_l, Qplus_0_l, Qminus_0_r, Qmult_1_l.
+      eapply IHt2 with (l:=l); auto.
+      * eapply in_not_bound_choice2; eauto.
+      * rewrite sum_Q_list_proper; eauto.
+        unfold flip; intros ?; simpl; rewrite q0; lra.
+    + destruct (Qeq_dec q 1).
+      * rewrite q0. rewrite Qminus_cancel, Qmult_1_l, Qmult_0_l, Qplus_0_r.
+        eapply IHt1 with (l:=l); auto.
+        ++ eapply in_not_bound_choice1; eauto.
+        ++ rewrite sum_Q_list_proper; eauto.
+           unfold flip; intros ?; simpl; rewrite q0; lra.
+      * rewrite IHt1 with (l:=l), IHt2 with (l:=l); auto. lra.
+        ++ eapply in_not_bound_choice2; eauto.
+        ++ apply sum_Q_list_infer_fail_choice_r in Hsum; eauto; try lra.
+           ** eapply in_not_bound_choice1; eauto.
+           ** eapply in_not_bound_choice2; eauto.
+        ++ eapply in_not_bound_choice1; eauto.
+        ++ apply sum_Q_list_infer_fail_choice_l in Hsum; eauto; try lra.
+           ** eapply in_not_bound_choice1; eauto.
+           ** eapply in_not_bound_choice2; eauto.
+  - unfold flip in *; simpl in *.
+    inversion Hwf; inversion Hnotbound; subst.
+    destruct (Qeq_dec (infer_fail n t) 1).
+    { (* Hsum is contradictory because the sum must equal 0 *)
+      assert (sum_Q_list (map (fun y => infer_fail y t / (1 - infer_fail n t)) l) == 0).
+      { erewrite <- sum_Q_list_map_const_0. apply sum_Q_list_proper.
+        intro y. rewrite q, Qminus_cancel, Qdiv_0_den; reflexivity. }
+      lra. }
+    rewrite Qeq_bool_false; auto.
+    rewrite IHt with (l:=n::l); auto.
+    + apply Qdiv_0_num.
+    + intros x [Hin|Hin]; subst; auto.
+      apply Hin_notbound in Hin. inversion Hin; subst; auto.
+    + constructor; auto. intro HC. apply Hin_notbound in HC.
+      inversion HC; subst; congruence.
+    + simpl.
+      destruct (Qeq_dec (infer_fail n t) 1).
+      * rewrite sum_Q_list_proper in Hsum.
+        ++ rewrite sum_Q_list_map_const_0 in Hsum; lra.
+        ++ intros ?; rewrite q, Qminus_cancel, Qdiv_0_den; reflexivity.
+      * rewrite sum_Q_list_map_div_scalar in Hsum.
+        ++ rewrite Qplus_comm; apply Qlem_2; auto.
+        ++ generalize (@infer_fail_le_1 A t n H1 H2); intros; lra.
+Qed.
+
+Lemma infer_f_lib_fail {A : Type} (t : tree A) (f : A -> Q) (l : nat) :
+  wf_tree t ->
+  not_bound_in l t ->
+  infer_fail l t == 1 ->
+  infer_f_lib f t == 0.
+Proof.
+  intros Hwf Hnotbound Heq.
+  eapply infer_f_lib_fail_aux with (l0:=[l]); auto.
+  - intros x Hin. destruct Hin; subst; auto; contradiction.
+  - constructor; auto; constructor.
+  - apply Hnotbound.
+  - simpl; unfold flip; rewrite Heq; reflexivity.
+Qed.
+
 Lemma infer_f_fail_chain {A : Type} (t : tree A) (f : A -> Q) (l n : nat) :
   wf_tree' t ->
   not_bound_in l (tree_chain t l n) ->
@@ -1086,25 +1178,6 @@ Proof.
   - rewrite IHt; auto. rewrite IHt; auto. reflexivity.
 Qed.
 
-Lemma infer_lib_chain_geometric {A : Type} (t : tree A) (f : A -> Q) (l : nat) :
-  wf_tree' t ->
-  (forall n m : nat, free_in n t -> bound_in m t -> (n < m)%nat) ->
-  (free_in l t) ->
-  infer_f_lib' f ∘ tree_chain t l
-  ==f geometric_series (infer_f_lib f t) (infer_fail_lib l t).
-Proof.
-Admitted.
-
-Lemma infer_f_lib_supremum {A : Type} (t : tree A) (f : A -> Q) (l : nat) :
-  expectation f ->
-  wf_tree' t ->
-  (forall m, bound_in m t -> (l < m)%nat) -> (* implies l not bound in chain *)
-  (forall n m : nat, bound_in m t -> free_in n t -> (n < m)%nat) ->
-  infimum (infer_f_lib f t / (1 - infer_fail_lib l t))
-          (infer_f_lib' f ∘ tree_chain t l).
-Proof.
-Admitted.
-
 Lemma infer_fail_tree_bind_infer_f e t m :
   not_in m t ->
   wf_tree' t ->
@@ -1147,47 +1220,128 @@ Lemma infer_f_lib_bind_fail t e f m :
   infer_f_lib (fun st => if e st : bool then 0 else f st) t ==
   infer_f_lib f (tree_bind t (fun st => if e st then Fail St m else Leaf st)).
 Proof.
-(*   revert e f m. *)
-(*   induction t; intros e f m Hnotbound; *)
-(*     unfold tree_bind; simpl; inversion Hnotbound; subst. *)
-(*   - destruct (e a); reflexivity. *)
-(*   - reflexivity. *)
-(*   - rewrite IHt1, IHt2; eauto; reflexivity. *)
-(*   - rewrite IHt; eauto. *)
-(*     generalize (@not_bound_in_infer_fail_tree_bind t e n m (not_eq_sym H2) H3). *)
-(*     intro Heq; rewrite Heq; reflexivity. *)
-(* Qed. *)
-Admitted.
+  revert e f m.
+  induction t; intros e f m Hnotbound;
+    unfold tree_bind; simpl; inversion Hnotbound; subst.
+  - destruct (e a); reflexivity.
+  - reflexivity.
+  - rewrite IHt1, IHt2; eauto; reflexivity.
+  - destruct (Qeq_dec (infer_fail n t) 1).
+    + rewrite q; simpl.
+      destruct (Qeq_dec (infer_fail n (tree_bind t (fun x => if e x then Fail _ m else Leaf x))) 1).
+      * unfold tree_bind in q0; rewrite q0; reflexivity.
+      * rewrite not_bound_in_infer_fail_tree_bind in n0; auto; congruence.
+    + rewrite Qeq_bool_false; auto.
+      destruct (Qeq_dec (infer_fail n (tree_bind t (fun x => if e x then Fail _ m else Leaf x))) 1).
+      * rewrite not_bound_in_infer_fail_tree_bind in q; auto; congruence.
+      * rewrite Qeq_bool_false; auto.
+        rewrite IHt; eauto.
+        generalize (@not_bound_in_infer_fail_tree_bind t e n m (not_eq_sym H2) H3).
+        intro Heq; rewrite Heq; reflexivity.
+Qed.
+
+Instance Proper_infer_f {A : Type}
+  : Proper ((@f_Qeq A) ==> eq ==> Qeq) infer_f.
+Proof.
+  intros f g Hfeq ? t ?; subst; revert f g Hfeq.
+  induction t; intros f g Hfeq; simpl; auto.
+  - reflexivity.
+  - rewrite IHt1, IHt2; eauto; reflexivity.
+  - rewrite IHt; eauto; reflexivity.
+Qed.
 
 Lemma infer_f_proper {A : Type} (t : tree A) (f g : A -> Q) :
   f ==f g ->
   infer_f f t == infer_f g t.
-Proof.
-  induction t; unfold f_Qeq; simpl; intro Heq.
-  - apply Heq.
-  - reflexivity.
-  - rewrite IHt1, IHt2; auto; reflexivity.
-  - rewrite IHt; auto; reflexivity.
-Qed.
+Proof. intros; apply Proper_infer_f; auto. Qed.
 
-Lemma infer_f_lib'_bind {A B : Type} (f : B -> Q) (t : tree A) (k : A -> tree B) :
-  (forall n x, bound_in n t -> not_in n (k x)) ->
-  infer_f_lib' (infer_f_lib' f ∘ k) t == infer_f_lib' f (tree_bind t k).
-Admitted.
+Instance Proper_infer_f_lib {A : Type}
+  : Proper ((@f_Qeq A) ==> eq ==> Qeq) infer_f_lib.
+  intros f g Hfeq ? t ?; subst; revert f g Hfeq.
+  induction t; intros f g Hfeq; simpl; auto.
+  - reflexivity.
+  - rewrite IHt1, IHt2; eauto; reflexivity.
+  - destruct (Qeq_dec (infer_fail n t) 1).
+    + rewrite q; reflexivity.
+    + rewrite Qeq_bool_false; auto; rewrite IHt; eauto; reflexivity.
+Qed.
 
 Lemma infer_f_lib_proper {A : Type} (t : tree A) (f g : A -> Q) :
   f ==f g ->
   infer_f_lib f t == infer_f_lib g t.
-Admitted.
+Proof. intros; apply Proper_infer_f_lib; auto. Qed.
 
-Lemma infer_f_lib'_proper {A : Type} (t : tree A) (f g : A -> Q) :
-  f ==f g ->
-  infer_f_lib' f t == infer_f_lib' g t.
+Lemma all_support_true_infer_f (e : St -> bool) (f g : St -> Q) (t : tree St) :
+  wf_tree t ->
+  all_support (fun x => e x = true) t ->
+  infer_f (fun x => if e x then f x else g x) t ==
+  infer_f f t.
 Proof.
-(*   induction t; unfold f_Qeq; simpl; intro Heq. *)
-(*   - apply Heq. *)
+  induction t; intros Hwf Hsupp; inversion Hwf; subst; simpl.
+  - inversion Hsupp; subst. rewrite H0; reflexivity.
+  - reflexivity.
+  - inversion Hsupp; subst.
+    + rewrite H1, 2!Qmult_0_l, 2!Qplus_0_l, Qminus_0_r, 2!Qmult_1_l.
+      apply IHt2; auto.
+    + rewrite H1, Qmult_1_l, Qminus_cancel,
+      2!Qmult_0_l, Qmult_1_l, 2!Qplus_0_r.
+      apply IHt1; auto.
+    + rewrite IHt1, IHt2; auto; reflexivity.
+  - inversion Hsupp; subst.
+    rewrite IHt; auto; reflexivity.
+Qed.
+
+(* Lemma infer_f_bind_fail_f (e : exp) t f n : *)
+(*   not_bound_in n t -> *)
+(*   infer_f f (tree_bind t (fun x => if e x then Leaf x else Fail St n)) == *)
+(*   infer_f (fun x => if e x then f x else 0) t. *)
+(* Proof. *)
+(*   unfold tree_bind. *)
+(*   revert e f n. induction t; intros e f m Hnotbound; simpl. *)
+(*   - destruct (e a); reflexivity. *)
 (*   - reflexivity. *)
-(*   - rewrite IHt1, IHt2; auto; reflexivity. *)
-(*   - rewrite IHt; auto; reflexivity. *)
+(*   - inversion Hnotbound; subst; rewrite IHt1, IHt2; auto; reflexivity. *)
+(*   - inversion Hnotbound; subst. *)
+(*     rewrite IHt; auto. *)
+(*     generalize (@not_bound_in_infer_fail_tree_bind t e n m (not_eq_sym H2) H3). *)
+(*     intro Heq. rewrite Heq. reflexivity. *)
 (* Qed. *)
-Admitted.
+
+Lemma infer_f_bind_fail_f_neg (e : exp) t f n :
+  not_bound_in n t ->
+  infer_f f (tree_bind t (fun x => if e x then Fail St n else Leaf x)) ==
+  infer_f (fun x => if e x then 0 else f x) t.
+Proof.
+  unfold tree_bind.
+  revert e f n. induction t; intros e f m Hnotbound; simpl.
+  - destruct (e a); reflexivity.
+  - reflexivity.
+  - inversion Hnotbound; subst; rewrite IHt1, IHt2; auto; reflexivity.
+  - inversion Hnotbound; subst.
+    rewrite IHt; auto.
+    generalize (@not_bound_in_infer_fail_tree_bind t e n m (not_eq_sym H2) H3).
+    intro Heq; rewrite Heq; reflexivity.
+Qed.
+
+Lemma infer_f_lib_bind_fail_f_neg (e : exp) t f n :
+  not_bound_in n t ->
+  infer_f_lib f (tree_bind t (fun x => if e x then Fail St n else Leaf x)) ==
+  infer_f_lib (fun x => if e x then 0 else f x) t.
+Proof.
+  unfold tree_bind.
+  revert e f n. induction t; intros e f m Hnotbound; simpl.
+  - destruct (e a); reflexivity.
+  - reflexivity.
+  - inversion Hnotbound; subst; rewrite IHt1, IHt2; auto; reflexivity.
+  - inversion Hnotbound; subst.
+      generalize (@not_bound_in_infer_fail_tree_bind t e n m (not_eq_sym H2) H3).
+      intro Heq.
+    destruct (Qeq_dec (infer_fail n (join (fmap (fun x : St => if e x then Fail St m else Leaf x) t))) 1).
+    + rewrite <- Heq, q; simpl; rewrite q; reflexivity.
+    + rewrite Qeq_bool_false; auto.
+      destruct (Qeq_dec (infer_fail n t) 1).
+      { rewrite q in Heq. unfold tree_bind in Heq. congruence. }
+      rewrite Qeq_bool_false; auto.
+      rewrite IHt; auto.
+      rewrite Heq; reflexivity.
+Qed.
